\documentclass{article}
\linespread{2.0}
\usepackage{amsfonts}
\usepackage{mathtools}
\usepackage{systeme}
\usepackage{graphicx} % Required for inserting images


\begin{document}

[Cauchy Condensation Test] Let $\{a_k\}$ be a sequence such that:
\begin{enumerate}

\item $a_1\geq a_2\geq a_3\geq\cdots\geq a_k\geq a_{k+1}\geq\cdots$
\item $a_k\geq 0$ for all $k\in\mathbb{N}$
\end{enumerate}

Then the series $\sum_{k=1}^\infty a_k$ converges if and only if $\sum_{k=0}^\infty 2^ka_{2^k}$ converges.

$\newline$
Corollary: The series $\sum_{k=1}^\infty\frac{1}{k^p}$ converges if and only if $p>1$.

Proof: 

For any $k \in \mathbb{N}$, let $a_k \coloneqq \frac{1}{k^p} > 0$. It is easy to see that $a_k > a_{k+1}$.

Note the series:

$\sum\limits_{k=1}^{2^n}\frac{1}{k^p}$

$= \frac{1}{1^p} + \frac{1}{2^p} + \frac{1}{3^p} + \dots + \frac{1}{2^{np}}$

$\le \frac{1}{1^p} + \frac{1}{2^p} + \frac{1}{2^p} + \dots + \frac{1}{2^{n-1}p}$

$\le \frac{1}{1^p} + \frac{2}{2^p} + \dots + \frac{2^{n-1}}{2^{(n-1)p}} $

$\le \sum\limits_{k=0}^{n-1} 2^k a_{2^k} = \sum\limits_{k=0}^{n-1} \frac{1}{2^{k(p-1)}} $

Consider the series $\sum\limits_{k=0}^\infty 2^ka_{2^k} = \sum\limits_{k=0}^\infty \frac{2^k}{2^{kp}} = \sum\limits_{k=0}^\infty \frac{1}{2^{k(p-1)}}$.

If $p \le 1$, $\frac{1}{2^{k(p-1)}} \geq 1$, then by Comparison Test, $\sum\limits_{k=0}^\infty \frac{1}{2^{k(p-1)}}$ diverges.

So, by Cauchy Condensation Test, the series $\sum\limits_{k=1}^\infty\frac{1}{k^p}$ converges if and only if $p > 1$. $\square$

\end{document}
